theories/Eq/SSim0Theory.v
@@ -1,4 +1,6 @@
-From Coq Require Import Lia Basics Fin.
+From Coq Require Import
+     Lia Basics Fin
+     Logic.Eqdep.
 
 From Coinduction Require Import
      coinduction rel tactics.
@@ -16,6 +18,7 @@ From CTree Require Import
 From RelationAlgebra Require Export
      rel srel.
 
+Import CTree.
 Set Implicit Arguments.
 
 (* TODO: Decide where to set this *)
@@ -28,21 +31,30 @@ Arguments trans : simpl never.
 
 Module SSim0Notations.
 
-  Notation "t ≲ u" := (ssim0 t u) (at level 70).
-  Notation "t [≲] u" := (ss0 _ t u) (at level 79).
-  Notation "t {≲} u" := (t (ss0 _) t u) (at level 79).
-  Notation "t {{≲}} u" := (bt (ss0 _) t u) (at level 79).
+  Notation "t ≲ u" := (ssim0 eq t u) (at level 70).
+  Notation "t [≲] u" := (ss0 eq _ t u) (at level 79).
+  Notation "t {≲} u" := (t (ss0 eq) _ t u) (at level 79).
+  Notation "t {{≲}} u" := (bt (ss0 eq) _ t u) (at level 79).
+
+  Notation "t ( ≲ L ) u" := (ssim0 L t u) (at level 70).
+  Notation "t [ ≲ L ] u" := (ss0 L _ t u) (at level 79).
+  Notation "t { ≲ L } u" := (t (ss0 L) _ t u) (at level 79).
+  Notation "t {{ ≲ L }} u" := (bt (ss0 L) _ t u) (at level 79).
 
 End SSim0Notations.
 
+Import CTreeNotations.
 Import EquNotations.
 Import SBisimNotations.
 
 Section ssim0_theory.
 
-  Context {E : Type -> Type} {X : Type}.
-  Notation ss0 := (@ss0 E X).
-  Notation ssim0 := (@ssim0 E X).
+  Context {E C : Type -> Type} {X : Type}
+          {L: relation (@label E)}
+          {HasStuck: B0 -< C} {EqL: Equivalence L}.
+
+  Notation ss0 := (@ss0 E E C C X X _ _ L).
+  Notation ssim0 := (@ssim0 E E C C X X _ _ L).
   Notation sst0 := (coinduction.t ss0).
   Notation ssbt0 := (coinduction.bt ss0).
   Notation ssT0 := (coinduction.T ss0).
@@ -58,13 +70,17 @@ Various results on reflexivity and transitivity.
 
   Lemma square_sst0 : square <= sst0.
   Proof.
-    apply Coinduction.
+    apply Coinduction; cbn.
     intros R x z [y xy yz] l x' xx'.
-    destruct (xy _ _ xx') as [y' yy' x'y'].
-    destruct (yz _ _ yy') as [z' zz' y'z'].
-    exists z'. assumption.
+    destruct (xy _ _ xx') as (l' & y' & yy' & ? & ?).
+    destruct (yz _ _ yy') as (l'' & z' & zz' & ? & ?).
+    exists l'', z'.
+    split.
+    assumption.
+    split.
     apply (f_Tf ss0).
-    eexists; eauto.
+    exists y'; eauto.
+    transitivity l'; auto.
   Qed.
 
   #[global] Instance PreOrder_sst0 R : PreOrder (sst0 R).
@@ -86,7 +102,7 @@ of the companion).
 |*)
 
   #[global] Instance sbisim_clos_ssim0_goal :
-    Proper (sbisim ==> sbisim ==> flip impl) ssim0.
+    Proper (sbisim L ==> sbisim L ==> flip impl) ssim0.
   Proof.
     repeat intro.
     symmetry in H0. apply sbisim_ssim0 in H, H0.
@@ -94,13 +110,13 @@ of the companion).
   Qed.
 
   #[global] Instance sbisim_clos_ssim0_ctx :
-    Proper (sbisim ==> sbisim ==> impl) ssim0.
+    Proper (sbisim L ==> sbisim L ==> impl) ssim0.
   Proof.
     repeat intro. symmetry in H, H0. eapply sbisim_clos_ssim0_goal; eauto.
   Qed.
 
   #[global] Instance sbisim_clos_sst_goal RR :
-    Proper (sbisim ==> sbisim ==> flip impl) (sst0 RR).
+    Proper (sbisim L ==> sbisim L ==> flip impl) (sst0 RR).
   Proof.
     cbn; intros ? ? eq1 ? ? eq2 H.
     symmetry in eq2. apply sbisim_ssim0 in eq1, eq2.
@@ -109,7 +125,7 @@ of the companion).
   Qed.
 
   #[global] Instance sbisim_clos_sst_ctx RR :
-    Proper (sbisim ==> sbisim ==> impl) (sst0 RR).
+    Proper (sbisim L ==> sbisim L ==> impl) (sst0 RR).
   Proof.
     cbn; intros ? ? eq1 ? ? eq2 ?.
     rewrite <- eq1, <- eq2.
@@ -117,7 +133,7 @@ of the companion).
   Qed.
 
   #[global] Instance sbisim_clos_ssT_goal RR f :
-    Proper (sbisim ==> sbisim ==> flip impl) (ssT0 f RR).
+    Proper (sbisim L ==> sbisim L ==> flip impl) (ssT0 f RR).
   Proof.
     cbn; intros ? ? eq1 ? ? eq2 ?.
     symmetry in eq2. apply sbisim_ssim0 in eq1, eq2.
@@ -126,7 +142,7 @@ of the companion).
   Qed.
 
   #[global] Instance sbisim_clos_ssT_ctx RR f :
-    Proper (sbisim ==> sbisim ==> impl) (ssT0 f RR).
+    Proper (sbisim L ==> sbisim L ==> impl) (ssT0 f RR).
   Proof.
     cbn; intros ? ? eq1 ? ? eq2 ?.
     rewrite <- eq1, <- eq2.
@@ -139,15 +155,16 @@ Strong simulation up-to [equ] is valid
 |*)
   Lemma equ_clos_sst0 : equ_clos <= sst0.
   Proof.
-    apply Coinduction.
-    intros R t u EQ l t1 TR. cbn in EQ. inv EQ.
-    cbn in *. rewrite Equt in TR.
-    apply HR in TR.
-    destruct TR.
-    exists x.
-    rewrite <- Equu; auto.
-    eapply (f_Tf ss0).
-    econstructor; auto; auto.
+    apply Coinduction; cbn.
+    intros R x y [x' y' x'' y'' EQ' EQ''] l z x'z.
+    rewrite EQ' in x'z.
+    destruct (EQ'' _ _ x'z) as (l' & ? & ? & ? & ?).
+    exists l', x0.
+    split.
+    - rewrite <- Equu; auto.
+    - split; auto.
+      eapply (f_Tf ss0).
+      econstructor; auto; auto.
   Qed.
 
   #[global] Instance equ_clos_sst0_goal RR :
@@ -209,50 +226,50 @@ Strong simulation up-to [equ] is valid
   #[global] Instance equ_ss0_closed_goal {r} : Proper (equ eq ==> equ eq ==> flip impl) (ss0 r).
   Proof.
     intros t t' tt' u u' uu'; cbn; intros.
-    rewrite tt' in H0. apply H in H0 as [? ? ?].
-    eexists; eauto. rewrite uu'. eauto.
+    rewrite tt' in H0. apply H in H0 as (l' & ? & ? & ? & ?).
+    do 2 eexists; eauto. rewrite uu'. eauto.
   Qed.
 
   #[global] Instance equ_ss0_closed_ctx {r} : Proper (equ eq ==> equ eq ==> impl) (ss0 r).
   Proof.
     intros t t' tt' u u' uu'; cbn; intros.
-    rewrite <- tt' in H0. apply H in H0 as [? ? ?].
-    eexists; eauto. rewrite <- uu'. eauto.
+    rewrite <- tt' in H0. apply H in H0 as (l' & ? & ? & ? & ?).
+    do 2 eexists; eauto. rewrite <- uu'. eauto.
   Qed.
 
-(*|
-stuck ctrees can be simulated by anything.
-|*)
-
-  Lemma is_stuck_ss0 (R : rel _ _) (t t' : ctree E X) :
+  (*|
+    stuck ctrees can be simulated by anything.
+    |*)
+  Lemma is_stuck_ss0 (R : rel _ _) (t t' : ctree E C X) :
     is_stuck t -> ss0 R t t'.
   Proof.
     repeat intro. now apply H in H0.
   Qed.
 
-  Lemma is_stuck_ssim0 (t t' : ctree E X) :
+  Lemma is_stuck_ssim0 (t t' : ctree E C X) :
     is_stuck t -> ssim0 t t'.
   Proof.
     intros. step. now apply is_stuck_ss0.
   Qed.
 
-  Lemma stuckD_ss0 (R : rel _ _) (t : ctree E X) : ss0 R CTree.stuckD t.
+  Lemma stuckD_ss0 (R : rel _ _) (t : ctree E C X) : ss0 R stuckD t.
   Proof.
     repeat intro. now apply stuckD_is_stuck in H.
   Qed.
 
-  Lemma stuckD_ssim0 (t : ctree E X) : ssim0 CTree.stuckD t.
+  Lemma stuckD_ssim0 (t : ctree E C X) : ssim0 stuckD t.
   Proof.
     intros. step. apply stuckD_ss0.
   Qed.
 
-  Lemma spinD_ss0 (R : rel _ _) (t : ctree E X) : ss0 R CTree.spinD t.
+  
+  Lemma spinD_ss0 (R : rel _ _) (t : ctree E C X) `{HasTau: B1 -< C}: ss0 R spinD t.
   Proof.
     repeat intro. now apply spinD_is_stuck in H.
   Qed.
 
-  Lemma spinD_ssim0 : forall (t' : ctree E X),
-      ssim0 CTree.spinD t'.
+  Lemma spinD_ssim0 : forall (t' : ctree E C X) `{HasTau: B1 -< C},
+      ssim0 spinD t'.
   Proof.
     intros. step. apply spinD_ss0.
   Qed.
@@ -272,24 +289,26 @@ We now prove the same result, but for strong simulation.
 Section bind.
   Obligation Tactic := idtac.
 
- Context {E : Type -> Type} {X Y : Type}.
+  Context {E C: Type -> Type} {X Y : Type}
+          {HasStuck: B0 -< C}.
 
 (*|
 Specialization of [bind_ctx] to a function acting with [ssim] on the bound value,
 and with the argument (pointwise) on the continuation.
 |*)
-  Program Definition bind_ctx_ssim0 : mon (rel (ctree E Y) (ctree E Y)) :=
-    {|body := fun R => @bind_ctx E X X Y Y ssim0 (pointwise eq R) |}.
+  Program Definition bind_ctx_ssim0 : mon (rel (ctree E C Y) (ctree E C Y)) :=
+    {|body := fun R => @bind_ctx E E C C X X Y Y (ssim0 eq) (pointwise eq R) |}.
   Next Obligation.
     intros ?? H. apply leq_bind_ctx. intros ?? H' ?? H''.
     apply in_bind_ctx. apply H'. intros t t' HS. apply H, H'', HS.
   Qed.
 
+  (* LEF: Make parametric on `L` *)
 (*|
 The resulting enhancing function gives a valid up-to technique
 |*)
   Lemma bind_ctx_ssim0_t :
-    bind_ctx_ssim0 <= sst0.
+    bind_ctx_ssim0 <= (sst0 eq).
   Proof.
     intro HL.
     apply Coinduction.
@@ -298,43 +317,43 @@ The resulting enhancing function gives a valid up-to technique
     step in tt.
     intros l u STEP.
     apply trans_bind_inv in STEP as [(H & t' & STEP & EQ) | (v & STEPres & STEP)]; cbn in *.
-    - apply tt in STEP as [u' STEP EQ'].
-      eexists.
-      apply trans_bind_l; eauto.
-      apply (fT_T equ_clos_sst0).
-      econstructor; [exact EQ | | reflexivity].
-      apply (fTf_Tf ss0).
-      apply in_bind_ctx; auto.
-      intros ? ? ->.
-      apply (b_T ss0).
-      red in kk. red. red. now apply kk.
-    - apply tt in STEPres as [u' STEPres EQ'].
+    - apply tt in STEP as (l' & u' & STEP & ? & EQ'); subst.
+      do 2 eexists; split.
+      + eapply trans_bind_l; eauto.
+      + split.
+        apply (fT_T equ_clos_sst0).
+        econstructor; [exact EQ | | reflexivity].
+        apply (fTf_Tf (ss0 eq)).
+        apply in_bind_ctx; auto.
+        intros ? ? ->.
+        apply (b_T (ss0 eq)).
+        red in kk. red. red. now apply kk. reflexivity.
+    - apply tt in STEPres as (l' & u' & STEPres & ? & ?); subst.
       pose proof (trans_val_inv STEPres) as EQ.
       rewrite EQ in STEPres.
       specialize (kk v v eq_refl).
-      apply kk in STEP as [u'' STEP EQ'']; cbn in *.
-      eexists.
-      eapply trans_bind_r; cbn in *; eauto.
-      eapply (id_T ss0); auto.
+      apply kk in STEP as (l'' & u'' & STEP & ? & EQ''); subst; cbn in *.
+      do 2 eexists.
+      split.
+      + eapply trans_bind_r; cbn in *; eauto.
+      + split. eapply (id_T (ss0 eq)); auto.
+        reflexivity.
   Qed.
 
 End bind.
 
-Import CTree.
-Import CTreeNotations.
-
 (*|
 Expliciting the reasoning rule provided by the up-to principles.
 |*)
-Lemma sst_clo_bind (E : Type -> Type) (X Y : Type) :
-  forall (t1 t2 : ctree E X) (k1 k2 : X -> ctree E Y) RR,
+Lemma sst_clo_bind (E C : Type -> Type) (X Y : Type) :
+  forall (t1 t2 : ctree E C X) (k1 k2 : X -> ctree E C Y) RR `{HasStuck: B0 -< C},
 		t1 ≲ t2 ->
-    (forall x, (sst0 RR) (k1 x) (k2 x)) ->
-    sst0 RR (t1 >>= k1) (t2 >>= k2)
+    (forall x, (sst0 eq RR) (k1 x) (k2 x)) ->
+    sst0 eq RR (t1 >>= k1) (t2 >>= k2)
 .
 Proof.
   intros.
-  apply (ft_t (@bind_ctx_ssim0_t E X Y)).
+  apply (ft_t (@bind_ctx_ssim0_t E C X Y _)).
   apply in_bind_ctx; auto.
   intros ? ? <-; auto.
 Qed.
@@ -342,15 +361,15 @@ Qed.
 (*|
 Specializing the congruence principle for [≲]
 |*)
-Lemma ssim0_clo_bind (E : Type -> Type) (X Y : Type) :
-  forall (t1 t2 : ctree E X) (k1 k2 : X -> ctree E Y),
+Lemma ssim0_clo_bind (E C: Type -> Type) (X Y : Type) :
+  forall (t1 t2 : ctree E C X) (k1 k2 : X -> ctree E C Y) `{HasStuck: B0 -< C},
 		t1 ≲ t2 ->
     (forall x, k1 x ≲ k2 x) ->
     t1 >>= k1 ≲ t2 >>= k2
 .
 Proof.
   intros * EQ EQs.
-  apply (ft_t (@bind_ctx_ssim0_t E X Y)).
+  apply (ft_t (@bind_ctx_ssim0_t E C X Y _)).
   apply in_bind_ctx; auto.
   intros ? ? <-; auto.
   apply EQs.
@@ -359,25 +378,27 @@ Qed.
 (*|
 And in particular, we can justify rewriting [≲] to the left of a [bind].
 |*)
-Lemma bind_ssim0_cong_gen {E X Y} RR :
-  Proper (ssim0 ==> pointwise_relation X (sst0 RR) ==> sst0 RR) (@bind E X Y).
+Lemma bind_ssim0_cong_gen {E C X Y} RR {HasStuck: B0 -< C}:
+  Proper (ssim0 eq ==> pointwise_relation X (sst0 eq RR) ==> sst0 eq RR) (@bind E C X Y).
+
 Proof.
   repeat red; intros; eapply sst_clo_bind; eauto.
 Qed.
 
 Ltac __upto_bind_ssim0 :=
   match goal with
-    |- @ssim0 _ ?X (CTree.bind (T := ?T) _ _) (CTree.bind (T := ?T') _ _) =>
+    |- @ssim0 ?E ?F ?C ?D ?X ?Y _ _ (CTree.bind (T := ?T) _ _) (CTree.bind (T := ?T') _ _) =>
       apply ssim0_clo_bind
-  | |- body (t (@ss0 ?E ?X)) ?R (CTree.bind (T := ?T) _ _) (CTree.bind (T := ?T) _ _) =>
-      apply (ft_t (@bind_ctx_ssim0_t E T X)), in_bind_ctx
-  | |- body (bt (@ss0 ?E ?X)) ?R (CTree.bind (T := ?T) _ _) (CTree.bind (T := ?T) _ _) =>
-      apply (fbt_bt (@bind_ctx_ssim0_t E T X)), in_bind_ctx
+  | |- body (t (@ss0 ?E ?F ?C ?D ?X ?Y _ _)) ?R (CTree.bind (T := ?T) _ _) (CTree.bind (T := ?T) _ _) =>
+      apply (ft_t (@bind_ctx_ssim0_t E C T X _)), in_bind_ctx
+  | |- body (bt (@ss0 ?E ?F ?C ?D ?X ?Y _ _)) ?R (CTree.bind (T := ?T) _ _) (CTree.bind (T := ?T) _ _) =>
+      apply (fbt_bt (@bind_ctx_ssim0_t E C T X _)), in_bind_ctx
   end.
+
 Ltac __upto_bind_eq_ssim0 :=
   match goal with
-  | |- @ssim0 _ ?X (CTree.bind (T := ?T) _ _) (CTree.bind (T := ?T') _ _) =>
-    __upto_bind_ssim0; [reflexivity | intros ?]
+  | |- @ssim0 ?E ?F ?C ?D ?X ?Y _ _ (CTree.bind (T := ?T) _ _) (CTree.bind (T := ?T') _ _) =>
+      __upto_bind_ssim0; [reflexivity | intros ?]
   | _ => __upto_bind_ssim0; [reflexivity | intros ? ? <-]
   end.
 
@@ -390,7 +411,7 @@ Ltac __play_ssim0_in H :=
 
 Ltac __eplay_ssim0 :=
   match goal with
-  | h : @ssim0 ?E ?X _ _ |- _ =>
+  | h : @ssim0 ?E _ ?C _ ?X _ _ _ ?L _ _ |- _ =>
       __play_ssim0_in h
   end.
 
@@ -400,147 +421,142 @@ Ltac __eplay_ssim0 :=
 
 Section Proof_Rules.
 
-  Context {E : Type -> Type}.
-  Context {X Y : Type}.
+  Context {E C: Type -> Type} {X Y : Type} {HasStuck: B0 -< C}.
 
   Lemma step_ss0_ret_gen (x y : X) (R : rel _ _) :
     R stuckD stuckD ->
     (Proper (equ eq ==> equ eq ==> impl) R) ->
     x = y ->
-    ss0 R (Ret x : ctree E X) (Ret y).
+    ss0 eq R (Ret x : ctree E C X) (Ret y).
   Proof.
     intros Rstuck PROP <-.
     cbn; intros ? ? TR; inv_trans; subst.
-    cbn; eexists; etrans.
-    now rewrite EQ.
+    cbn; do 2 eexists. 
+    split.
+    - etrans.
+    - split. now rewrite EQ. reflexivity.
   Qed.
 
   Lemma step_ss0_ret (x y : X) (R : rel _ _) :
     x = y ->
-    ssbt0 R (Ret x : ctree E X) (Ret y).
+    ssbt0 eq R (Ret x : ctree E C X) (Ret y).
   Proof.
     apply step_ss0_ret_gen.
     reflexivity.
     typeclasses eauto.
   Qed.
 
-(*|
-The vis nodes are deterministic from the perspective of the labeled transition system,
-stepping is hence symmetric and we can just recover the itree-style rule.
-|*)
-  Lemma step_ss0_vis_gen (e : E X) (k k' : X -> ctree E Y) (R : rel _ _) :
+  (*|
+    The vis nodes are deterministic from the perspective of the labeled transition system,
+    stepping is hence symmetric and we can just recover the itree-style rule.
+    |*)
+  Lemma step_ss0_vis_gen (e : E X) (k k' : X -> ctree E C Y) (R : rel _ _) :
     (Proper (equ eq ==> equ eq ==> impl) R) ->
     (forall x, R (k x) (k' x)) ->
-    ss0 R (Vis e k) (Vis e k').
+    ss0 eq R (Vis e k) (Vis e k').
   Proof.
     intros PR EQs.
     intros ? ? TR; inv_trans; subst.
-    cbn; eexists; etrans. rewrite EQ; auto.
+    cbn; do 2 eexists; split; [etrans | split; [rewrite EQ; eauto|reflexivity]].
   Qed.
 
-  Lemma step_ss0_vis (e : E X) (k k' : X -> ctree E Y) (R : rel _ _) :
-    (forall x, sst0 R (k x) (k' x)) ->
-    ssbt0 R (Vis e k) (Vis e k').
+  Lemma step_ss0_vis (e : E X) (k k' : X -> ctree E C Y) (R : rel _ _) :
+    (forall x, sst0 eq R (k x) (k' x)) ->
+    ssbt0 eq R (Vis e k) (Vis e k').
   Proof.
     intros * EQ.
     apply step_ss0_vis_gen; auto.
     typeclasses eauto.
   Qed.
 
-(*|
-Same goes for visible tau nodes.
-|*)
-   Lemma step_ss0_step_gen (t t' : ctree E X) (R : rel _ _) :
+  (*|
+    Same goes for visible tau nodes.
+    |*)
+   Lemma step_ss0_step_gen (t t' : ctree E C X) (R : rel _ _) {HasTau: B1 -< C}:
     (Proper (equ eq ==> equ eq ==> impl) R) ->
     (R t t') ->
-    ss0 R (Step t) (Step t').
+    ss0 eq R (Step t) (Step t').
   Proof.
     intros PR EQs.
     intros ? ? TR; inv_trans; subst.
-    cbn; eexists; etrans; rewrite EQ; auto.
+    cbn; do 2 eexists; split; [etrans | split; [rewrite EQ; eauto|reflexivity]].
   Qed.
 
-  Lemma step_ss0_step (t t' : ctree E X) (R : rel _ _) :
-    (sst0 R t t') ->
-    ssbt0 R (Step t) (Step t').
+  Lemma step_ss0_step (t t' : ctree E C X) (R : rel _ _) {HasTau: B1 -< C}:
+    (sst0 eq R t t') ->
+    ssbt0 eq R (Step t) (Step t').
   Proof.
     intros. apply step_ss0_step_gen; auto.
     typeclasses eauto.
   Qed.
 
-(*|
-When matching visible brs one against another, in general we need to explain how
-we map the branches from the left to the branches to the right.
-A useful special case is the one where the arity coincide and we simply use the identity
-in both directions. We can in this case have [n] rather than [2n] obligations.
-|*)
-
-  Lemma step_ss0_brS_gen n m (k : fin n -> ctree E X) (k' : fin m -> ctree E X) (R : rel _ _) :
+  (*|
+    When matching visible brs one against another, in general we need to explain how
+    we map the branches from the left to the branches to the right.
+    A useful special case is the one where the arity coincide and we simply use the identity
+    in both directions. We can in this case have [n] rather than [2n] obligations.
+    |*)
+  Lemma step_ss0_brS_gen Z (c : C Y) (c' : C Z) (k : Y -> ctree E C X) (k' : Z -> ctree E C X) (R : rel _ _) :
     (Proper (equ eq ==> equ eq ==> impl) R) ->
     (forall x, exists y, R (k x) (k' y)) ->
-    ss0 R (BrS n k) (BrS m k').
+    ss0 eq R (BrS c k) (BrS c' k').
   Proof.
     intros PROP EQs ? ? TR; inv_trans; subst.
     destruct (EQs x) as [y HR].
-    eexists.
-    etrans.
-    rewrite EQ; eauto.
+    cbn; do 2 eexists; split; [etrans | split; [rewrite EQ; eauto|reflexivity]].
   Qed.
 
-  Lemma step_ss0_brS n m (k : fin n -> ctree E X) (k' : fin m -> ctree E X) (R : rel _ _) :
-    (forall x, exists y, sst0 R (k x) (k' y)) ->
-    ssbt0 R (BrS n k) (BrS m k').
+  Lemma step_ss0_brS Z (c : C Y) (c' : C Z) (k : Y -> ctree E C X) (k' : Z -> ctree E C X) (R : rel _ _) :
+    (forall x, exists y, sst0 eq R (k x) (k' y)) ->
+    ssbt0 eq R (BrS c k) (BrS c' k').
   Proof.
-    intros ? EQs.
+    intros.    
     apply step_ss0_brS_gen; auto.
     typeclasses eauto.
   Qed.
 
-  Lemma step_ss0_brS_id_gen n
-    (k k' : fin n -> ctree E X) (R : rel _ _) :
+  Lemma step_ss0_brS_id_gen (c : C Y) (k k' : Y -> ctree E C X) (R : rel _ _) :
     (Proper (equ eq ==> equ eq ==> impl) R) ->
     (forall x, R (k x) (k' x)) ->
-    ss0 R (BrS n k) (BrS n k').
+    ss0 eq R (BrS c k) (BrS c k').
   Proof.
-    intros PROP ? EQs.
-    apply step_ss0_brS_gen; auto.
-    intros x; exists x; auto.
+    intros; apply step_ss0_brS_gen; eauto.
   Qed.
-
-  Lemma step_ss0_brS_id n
-    (k k' : fin n -> ctree E X) (R : rel _ _) :
-    (forall x, sst0 R (k x) (k' x)) ->
-    ssbt0 R (BrS n k) (BrS n k').
+  
+  Lemma step_ss0_brS_id (c : C Y) (k k' : Y -> ctree E C X) (R : rel _ _) :
+    (forall x, sst0 eq R (k x) (k' x)) ->
+    ssbt0 eq R (BrS c k) (BrS c k').
   Proof.
+    intros.
     apply step_ss0_brS_id_gen.
     typeclasses eauto.
+    eauto.
   Qed.
 
-(*|
-For invisible nodes, the situation is different: we may kill them, but that execution
-cannot act as going under the guard.
-|*)
-  Lemma step_ss0_tauI_gen (t t' : ctree E X) (R : rel _ _) :
-    ss0 R t t' ->
-    ss0 R (Guard t) (Guard t').
+  (*|
+    For invisible nodes, the situation is different: we may kill them, but that execution
+    cannot act as going under the guard.
+    |*)
+  Lemma step_ss0_guard_gen (t t' : ctree E C X) (R : rel _ _) {HasTau: B1 -< C}:
+    ss0 eq R t t' ->
+    ss0 eq R (Guard t) (Guard t').
   Proof.
     intros EQ.
     intros ? ? TR; inv_trans; subst.
-    apply EQ in TR as [? ? ?].
-    etrans.
+    apply EQ in TR as (? & ? & ? & ? & ?); subst.
+    do 2 eexists; split; [etrans | split; trivial].
   Qed.
 
-  Lemma step_ss0_tauI (t t' : ctree E X) (R : rel _ _) :
-    ssbt0 R t t' ->
-    ssbt0 R (Guard t) (Guard t').
+  Lemma step_ss0_guard (t t' : ctree E C X) (R : rel _ _) {HasTau: B1 -< C} :
+    ssbt0 eq R t t' ->
+    ssbt0 eq R (Guard t) (Guard t').
   Proof.
-    apply step_ss0_tauI_gen.
+    apply step_ss0_guard_gen.
   Qed.
 
-  Lemma step_ss0_brD_l_gen n
-    (k : fin n -> ctree E X) (t' : ctree E X) (R : rel _ _) :
-    (forall x, ss0 R (k x) t') ->
-    ss0 R (BrD n k) t'.
+  Lemma step_ss0_brD_l_gen n (c : C n) (k : n -> ctree E C X) (t': ctree E C X) (R: rel _ _):
+    (forall x, ss0 eq R (k x) t') ->
+    ss0 eq R (BrD c k) t'.
   Proof.
     intros EQs.
     intros ? ? TR; inv_trans; subst.
@@ -548,36 +564,34 @@ cannot act as going under the guard.
     eauto.
   Qed.
 
-  Lemma step_ss0_brD_l n
-    (k : fin n -> ctree E X) (t' : ctree E X) (R : rel _ _) :
-    (forall x, ssbt0 R (k x) t') ->
-    ssbt0 R (BrD n k) t'.
+  Lemma step_ss0_brD_l n (c : C n) 
+    (k : n -> ctree E C X) (t' : ctree E C X) (R : rel _ _) :
+    (forall x, ssbt0 eq R (k x) t') ->
+    ssbt0 eq R (BrD c k) t'.
   Proof.
     apply step_ss0_brD_l_gen.
   Qed.
 
-  Lemma step_ss0_brD_r_gen :
-    forall (t : ctree E X) n (k : fin n -> ctree E X) x R,
-    ss0 R t (k x) ->
-    ss0 R t (BrD n k).
+  Lemma step_ss0_brD_r_gen n (c: C n) (k : n -> ctree E C X) (t: ctree E C X) x R:
+    ss0 eq R t (k x) ->
+    ss0 eq R t (BrD c k).
   Proof.
     cbn. intros.
-    apply H in H0 as [? ? ?].
+    apply H in H0 as (? & ? & ? & ? & ?).
     exists x0; etrans.
   Qed.
 
-  Lemma step_ss0_brD_r :
-    forall (t : ctree E X) n (k : fin n -> ctree E X) x R,
-    ssbt0 R t (k x) ->
-    ssbt0 R t (BrD n k).
+  Lemma step_ss0_brD_r n (c: C n) (k : n -> ctree E C X) (t: ctree E C X) x R:
+    ssbt0 eq R t (k x) ->
+    ssbt0 eq R t (BrD c k).
   Proof.
     intros. eapply step_ss0_brD_r_gen. apply H.
   Qed.
 
-  Lemma step_ss0_brD_gen n m
-    (k : fin n -> ctree E X) (k' : fin m -> ctree E X) (R : rel _ _) :
-    (forall x, exists y, ss0 R (k x) (k' y)) ->
-    ss0 R (BrD n k) (BrD m k').
+  Lemma step_ss0_brD_gen n m (cn: C n) (cm: C m)
+    (k : n -> ctree E C X) (k' : m -> ctree E C X) (R : rel _ _) :
+    (forall x, exists y, ss0 eq R (k x) (k' y)) ->
+    ss0 eq R (BrD cn k) (BrD cm k').
   Proof.
     intros EQs.
     apply step_ss0_brD_l_gen.
@@ -585,27 +599,27 @@ cannot act as going under the guard.
     now apply step_ss0_brD_r_gen with (x := x').
   Qed.
 
-  Lemma step_ss0_brD n m
-    (k : fin n -> ctree E X) (k' : fin m -> ctree E X) (R : rel _ _) :
-    (forall x, exists y, ssbt0 R (k x) (k' y)) ->
-    ssbt0 R (BrD n k) (BrD m k').
+  Lemma step_ss0_brD n m (cn: C n) (cm: C m)
+    (k : n -> ctree E C X) (k' : m -> ctree E C X) (R : rel _ _) :
+    (forall x, exists y, ssbt0 eq R (k x) (k' y)) ->
+    ssbt0 eq R (BrD cn k) (BrD cm k').
   Proof.
     apply step_ss0_brD_gen.
   Qed.
 
-  Lemma step_ss0_brD_id_gen n
-    (k k' : fin n -> ctree E X) (R : rel _ _) :
-    (forall x, ss0 R (k x) (k' x)) ->
-    ss0 R (BrD n k) (BrD n k').
+  Lemma step_ss0_brD_id_gen n (c: C n)
+    (k k' : n -> ctree E C X) (R : rel _ _) :
+    (forall x, ss0 eq R (k x) (k' x)) ->
+    ss0 eq R (BrD c k) (BrD c k').
   Proof.
     intros; apply step_ss0_brD_gen.
     intros x; exists x; apply H.
   Qed.
 
-  Lemma step_ss0_brD_id n
-    (k k' : fin n -> ctree E X) (R : rel _ _) :
-    (forall x, ssbt0 R (k x) (k' x)) ->
-    ssbt0 R (BrD n k) (BrD n k').
+  Lemma step_ss0_brD_id n (c: C n)
+    (k k' : n -> ctree E C X) (R : rel _ _) :
+    (forall x, ssbt0 eq R (k x) (k' x)) ->
+    ssbt0 eq R (BrD c k) (BrD c k').
   Proof.
     apply step_ss0_brD_id_gen.
   Qed.
@@ -614,120 +628,127 @@ End Proof_Rules.
 
 Section WithParams.
 
-  Context {E : Type -> Type}.
-  Context {X : Type}.
+  Context {E C: Type -> Type} {X : Type} {HasStuck: B0 -< C}.
 
-(*|
-Note that with visible schedules, nary-spins are equivalent only
-if neither are empty, or if both are empty: they match each other's
-tau challenge infinitely often.
-With invisible schedules, they are always equivalent: neither of them
-produce any challenge for the other.
-|*)
-  Lemma spinS_nary_n_m : forall n m,
-    n > 0 -> m > 0 ->
-    ssim0 (@spinS_nary E X n) (spinS_nary m).
+  (*|
+    Note that with visible schedules, nary-spins are equivalent only
+    if neither are empty, or if both are empty: they match each other's
+    tau challenge infinitely often.
+    With invisible schedules, they are always equivalent: neither of them
+    produce any challenge for the other.
+  |*)
+  Lemma spinS_gen_nonempty : forall {Z X Y} (c: C X) (c': C Y) (x: X) (y: Y),
+      @spinS_gen E C Z X c ≲ @spinS_gen E C Z Y c'.
   Proof.
-    intros.
-    red. coinduction R CH.
-    intros l t' TR.
-    destruct m as [|m]; [lia |].
-    rewrite ctree_eta in TR; cbn in TR.
-    apply trans_brS_inv in TR as (_ & EQ & ->).
-    eexists.
-    rewrite ctree_eta; cbn.
-    econstructor. exact Fin.F1.
-    reflexivity.
-    rewrite EQ; auto.
+    intros R.
+    coinduction S CIH; cbn; intros ? ? ? ? ? ? ? ? TR.
+      rewrite ctree_eta in TR; cbn in TR;
+      apply trans_brS_inv in TR as (_ & EQ & ->);
+      eexists; eexists;
+      rewrite ctree_eta; cbn.
+      split; [econstructor|].
+      + exact y.
+      + reflexivity.
+      + rewrite EQ; eauto.
   Qed.
+   
 
-(*|
-Inversion principles
---------------------
-|*)
+
+  (*|
+    Inversion principles
+    --------------------
+    |*)
   Lemma ssim0_ret_inv (r1 r2 : X) :
-    (Ret r1 : ctree E X) ≲ Ret r2 ->
+    (Ret r1 : ctree E C X) ≲ Ret r2 ->
     r1 = r2.
   Proof.
     intro.
-    eplay. etrans. inv_trans. auto.
+    eplay.
+    destruct TR as (? & ? & ? & <-).
+    now inv_trans.    
   Qed.
 
   Lemma ssim0_vis_inv_type {X1 X2}
-        (e1 : E X1) (e2 : E X2) (k1 : X1 -> ctree E X) (k2 : X2 -> ctree E X) (x : X1):
+        (e1 : E X1) (e2 : E X2) (k1 : X1 -> ctree E C X) (k2 : X2 -> ctree E C X) (x : X1):
     Vis e1 k1 ≲ Vis e2 k2 ->
     X1 = X2.
   Proof.
     intros.
     eplay.
-    inv TR; auto.
-    Unshelve. auto.
+    destruct TR as (? & ? & ? & <-).
+    inv_trans. inv EQl; eauto.
+    Unshelve. exact x.
   Qed.
 
-  Lemma ssbt0_eq_vis_inv {Y} (e1 e2 : E Y) (k1 k2 : Y -> ctree E X) (x : Y) R :
-    ssbt0 R (Vis e1 k1) (Vis e2 k2) ->
-    e1 = e2 /\ forall x, sst0 R (k1 x) (k2 x).
+  Lemma ssbt0_eq_vis_inv {Y} (e1 e2 : E Y) (k1 k2 : Y -> ctree E C X) (x : Y) R :
+    ssbt0 eq R (Vis e1 k1) (Vis e2 k2) ->
+    e1 = e2 /\ forall x, sst0 eq R (k1 x) (k2 x).
   Proof.
     intros.
     split.
-    - cbn in H. edestruct H as [? ? ?].
-      etrans. subst. now inv_trans.
-    - cbn. intros. edestruct H as [? ? ?].
-      etrans. subst. inv_trans. subst. apply H1.
-    Unshelve. auto.
-  Qed.
+    - edestruct H as [? ? ?].
+      etrans. destruct H0 as (? & ? & ? & ?). subst. now inv_trans.
+    - intros.
+      edestruct H as [? ? ?].
+      etrans.
+      destruct H0 as (? & ? & ? & ?). subst. simpl in *.
+      inv H0. apply inj_pair2 in H4, H5,H6, H7; subst.
+      rewrite H3.
+      rewrite ctree_eta in H1; cbn in H1.
+  Admitted.
 
-  Lemma ssim0_eq_vis_inv {Y} (e1 e2 : E Y) (k1 k2 : Y -> ctree E X) (x : Y) :
+  Lemma ssim0_eq_vis_inv {Y} (e1 e2 : E Y) (k1 k2 : Y -> ctree E C X) (x : Y) :
     Vis e1 k1 ≲ Vis e2 k2 ->
     e1 = e2 /\ forall x, k1 x ≲ k2 x.
   Proof.
     intros.
     (* Why doesn't apply work directly here? *)
-    epose proof (proj1 (enhanced_gfp (@ss0 E X) _ _)). apply H0 in H. clear H0.
+    epose proof (proj1 (enhanced_gfp (@ss0 E E C C X X _ _ eq) _ _)). apply H0 in H. clear H0.
     step in H. apply ssbt0_eq_vis_inv in H; auto.
     destruct H. split; auto.
-    intro. subst. specialize (H0 x0).
-    apply (proj1 (t_gfp_bt (@ss0 E X) _ _)) in H0. apply H0.
+    intro. subst. specialize (H0 x0).    
+    apply (proj1 (t_gfp_bt (@ss0 E E C C X X _ _ eq) _ _)) in H0. apply H0.
   Qed.
 
   Lemma ssim0_brS_inv
-        n1 n2 (k1 : fin n1 -> ctree E X) (k2 : fin n2 -> ctree E X) :
-    BrS n1 k1 ≲ BrS n2 k2 ->
+        n m (cn: C n) (cm: C m) (k1 : n -> ctree E C X) (k2 : m -> ctree E C X) :
+    BrS cn k1 ≲ BrS cm k2 ->
     (forall i1, exists i2, k1 i1 ≲ k2 i2).
   Proof.
     intros EQ i1.
     eplay.
+    destruct TR as (? & ? & ? & ?); subst.
     inv_trans.
     eexists; eauto.
   Qed.
 
-  Lemma ss0_brD_l_inv : forall n
-    (t : ctree E X) (k : fin n -> ctree E X) R,
-    ss0 R (BrD n k) t ->
-    forall x, ss0 R (k x) t.
+  Lemma ss0_brD_l_inv n (c: C n)
+    (t : ctree E C X) (k : n -> ctree E C X) R:
+    ss0 eq R (BrD c k) t ->
+    forall x, ss0 eq R (k x) t.
   Proof.
     cbn. intros.
     eapply trans_brD in H0; [| reflexivity].
-    apply H in H0 as [? ? ?].
-    exists x0; auto.
+    apply H in H0 as (? & ? & ? & ? & ?); subst.
+    eauto.
   Qed.
 
-  Lemma ssim0_brD_l_inv : forall n
-    (t : ctree E X) (k : fin n -> ctree E X),
-    BrD n k ≲ t ->
+  Lemma ssim0_brD_l_inv n (c: C n)
+    (t : ctree E C X) (k : n -> ctree E C X):
+    BrD c k ≲ t ->
     forall x, k x ≲ t.
   Proof.
     intros. step. step in H. eapply ss0_brD_l_inv. apply H.
   Qed.
 
   (* This one isn't very convenient... *)
-  Lemma ssim0_brD_r_inv : forall n
-    (t : ctree E X) (k : fin n -> ctree E X),
-    t ≲ BrD n k ->
+  Lemma ssim0_brD_r_inv n (c: C n)
+    (t : ctree E C X) (k : n -> ctree E C X):
+    t ≲ BrD c k ->
     forall l t', trans l t t' ->
     exists x t'', trans l (k x) t'' /\ t' ≲ t''.
   Proof.
-    cbn. intros. step in H. apply H in H0 as [? ? ?]. inv_trans.
+    cbn. intros. step in H. apply H in H0 as (? & ? & ? & ? & ?); subst. inv_trans.
     eauto.
   Qed.
 
@@ -740,26 +761,34 @@ This property is true if we only allow brs with 0 or 1 branch,
 but we prove a counter-example for a ctree with a binary br.
 |*)
 
-Lemma ss0_sb : forall {E X} RR
-  (t t' : ctree E X),
-  ss0 RR t t' ->
-  ss0 (flip RR) t' t ->
-  sb RR t t'.
+Lemma ss0_sb : forall {E C X} RR {HasStuck: B0 -< C}
+  (t t' : ctree E C X),
+  ss0 eq RR t t' ->
+  ss0 eq (flip RR) t' t ->
+  sb eq RR t t'.
 Proof.
-  split; auto.
+  intros.
+  split; eauto.
+  simpl in *; intros.
+  destruct (H0 _ _ H1) as (? & ? & ? & ? & ?).
+  destruct (H _ _ H2) as (? & ? & ? & ? & ?).
+  subst; eauto.
 Qed.
 
-#[local] Definition t1 : ctree void1 unit :=
+#[local] Definition t1 : ctree void1 (B0 +' B1) unit :=
   Step (Ret tt).
 
-#[local] Definition t2 : ctree void1 unit :=
+#[local] Definition t2 : ctree void1 (B0 +' B2) unit :=
   brS2 (Ret tt) (stuckD).
 
 Lemma ssim0_hsbisim_nequiv :
-  ssim0 t1 t2 /\ ssim0 t2 t1 /\ ~ sbisim t1 t2.
+  ssim0 eq t1 t2 /\ ssim0 eq t2 t1 /\ ~ sbisim eq t1 t2.
 Proof.
   unfold t1, t2. intuition.
-  - step. apply step_ss0_brS; auto.
+  - step.
+Admitted.
+(* LEF: Hm, not sure how to work with the preorder of branch effects... 
+apply step_ss0_brS; auto.
     intros _. exists Fin.F1. reflexivity.
   - step. apply step_ss0_brS; auto.
     intro. exists Fin.F1. destruct x.
@@ -773,3 +802,4 @@ Proof.
     intro. destruct H1 as [? ? ?].
     now apply stuckD_is_stuck in H1.
 Qed.
+*)
